switch to subgroup from subgroup2

src/week_2/kb_solutions/Part_B_subgroups_solutions.lean
@@ -1,4 +1,4 @@
-import week_2.Part_A_groups
+import week_2.kb_solutions.Part_A_groups_solutions
 
 /-!
 
@@ -8,9 +8,11 @@ Lean has subgroups already, so we'll call ours subgroup2.
 
 -/
 
+namespace xena
+
 /-- A subgroup of a group G is a subset containing 1
 and closed under multiplication and inverse. -/
-structure subgroup2 (G : Type) [group2 G] :=
+structure subgroup (G : Type) [group G] :=
 (carrier : set G)
 (one_mem' : (1 : G) ∈ carrier)
 (mul_mem' {x y} : x ∈ carrier → y ∈ carrier → x * y ∈ carrier)
@@ -33,16 +35,16 @@ I want to write `H`. Let's start by sorting this out.
 
 -/
 
-namespace subgroup2
+namespace subgroup
 
-open group2
+open xena.group
 
 -- let G be a group and let H and K be subgroups
-variables {G : Type} [group2 G] (H K : subgroup2 G)
+variables {G : Type} [group G] (H K : subgroup G)
 
 -- If `x : G` and `H : subgroup2 G` then let's define `x ∈ H` to mean
 -- `x ∈ H.carrier`
-instance : has_mem G (subgroup2 G) := ⟨λ m H, m ∈ H.carrier⟩
+instance : has_mem G (subgroup G) := ⟨λ m H, m ∈ H.carrier⟩
 
 -- Now let's define theorems without the `'`s in, which use this
 -- more normal notation
@@ -82,13 +84,13 @@ Say `H : subgroup G`. Then:
 -/
 
 -- now we can prove basic theorems about subgroups using this sensible notation
--- Remember that `group2.inv_inv x` is the statement that `x⁻¹⁻¹ = x`
+-- Remember that `xena.group.inv_inv x` is the statement that `x⁻¹⁻¹ = x`
 
 @[simp] theorem inv_mem_iff {x :G} : x⁻¹ ∈ H ↔ x ∈ H := 
 begin
   split,
   { intro h,
-    rw ← group2.inv_inv x,
+    rw ← xena.group.inv_inv x,
     apply H.inv_mem,
     assumption },
   { apply H.inv_mem },
@@ -102,7 +104,7 @@ Let's prove variants of this triviality now.
 -/
 
 /-- Two subgroups are equal if the underlying subsets are equal. -/
-theorem ext' {H K : subgroup2 G} (h : H.carrier = K.carrier) : H = K :=
+theorem ext' {H K : subgroup G} (h : H.carrier = K.carrier) : H = K :=
 begin
   -- first take H and K apart
   cases H,
@@ -114,7 +116,7 @@ end
 -- here's a variant
 
 /-- Two subgroups are equal if and only if the underlying subsets are equal. -/
-protected theorem ext'_iff {H K : subgroup2 G} :
+protected theorem ext'_iff {H K : subgroup G} :
   H.carrier = K.carrier ↔ H = K :=
 begin
   split,
@@ -127,7 +129,7 @@ end
 -- and then use the `ext` tactic (which works on sets)
 
 /-- Two subgroups are equal if they have the same elements. -/
-@[ext] theorem ext {H K : subgroup2 G} (h : ∀ x, x ∈ H ↔ x ∈ K) : H = K :=
+@[ext] theorem ext {H K : subgroup G} (h : ∀ x, x ∈ H ↔ x ∈ K) : H = K :=
 begin
   -- first apply ext' to reduce to checking the carriers are equal
   apply ext',
@@ -139,43 +141,38 @@ begin
 end
 
 /-
-We tagged that theorem with `ext`, so now if you ever have a goal
-of proving that two subgroups are equal, you can apply the `ext`
-tactic to reduce to showing that they have the same elements.
+We tagged that theorem with `ext`, so now the `ext` tactic works on subgroups
+too: if you ever have a goal of proving that two subgroups are equal, you can
+use the `ext` tactic to reduce to showing that they have the same elements.
 -/
-
--- subgroups form a lattice -- MOVE TO LATER
-instance : has_le (subgroup2 G) := ⟨λ S T, S.carrier ⊆ T.carrier⟩
 
 -- Coersion to group
 -- Coercion from subgroup2 to underlying type
 
-instance : has_coe (subgroup2 G) (set G) := ⟨subgroup2.carrier⟩
+instance : has_coe (subgroup G) (set G) := ⟨subgroup.carrier⟩
 
-lemma mem_coe' {g : G} : g ∈ (H : set G) ↔ g ∈ H := iff.rfl
+--lemma mem_coe' {g : G} : g ∈ (H : set G) ↔ g ∈ H := iff.rfl
 
 
 
 /-
-Let G be a group. The type of subgroup2s of G is `subgroup2 G`. 
-In other words, if `H : subgroup2 G` then H is a subgroup2 of G. 
-The three basic facts you need to know about H are:
-
-H.one_mem : (1 : G) ∈ H
-H.mul_mem {x y : G} : x ∈ H → y ∈ H → x * y ∈ H
-H.inv_mem {x : G} : x ∈ H → x⁻¹ ∈ H
-
-Subgroup2s of a group form what is known as a *lattice*. 
+Subgroups of a group form what is known as a *lattice*. 
 This is a partially ordered set with a sensible notion of
-max and min (and even sup and inf). 
+max and min. Subgroups even have a good notion of an infinite
+sup and inf.
 
 We will prove this here.
+
+We start by defining a relation ≤ on the type of subgroups of a group.
+We say H ≤ K iff H.carrier ⊆ K.carrier .
 -/
+instance : has_le (subgroup G) := ⟨λ S T, S.carrier ⊆ T.carrier⟩
+
 
 open set
 
 -- The intersect of two subgroup2s is also a subgroup2
-def inf (H K : subgroup2 G) : subgroup2 G :=
+def inf (H K : subgroup G) : subgroup G :=
 { carrier := H.carrier ∩ K.carrier,
   one_mem' := ⟨H.one_mem, K.one_mem⟩,
   mul_mem' := λ _ _ ⟨hhx, hkx⟩ ⟨hhy, hky⟩, 
@@ -183,13 +180,13 @@ def inf (H K : subgroup2 G) : subgroup2 G :=
   inv_mem' := λ x ⟨hhx, hhy⟩,
   ⟨H.inv_mem hhx, K.inv_mem hhy⟩}
 
-lemma inf_def (H K : subgroup2 G) : (inf H K : set G) = (H : set G) ∩ K := rfl 
+lemma inf_def (H K : subgroup G) : (inf H K : set G) = (H : set G) ∩ K := rfl 
 
 /- 
 We will consider the closure of a set as the intersect of all subgroup2s
 containing the set
 -/
-instance : has_Inf (subgroup2 G) :=
+instance : has_Inf (subgroup G) :=
 ⟨λ s, {
   carrier := ⋂ t ∈ s, (t : set G),
   one_mem' := mem_bInter $ λ i h, i.one_mem,
@@ -199,10 +196,10 @@ instance : has_Inf (subgroup2 G) :=
   inv_mem' := λ x hx, mem_bInter $ λ i h,
     i.inv_mem (by apply mem_bInter_iff.1 hx i h) }⟩
 
-def closure (S : set G) : subgroup2 G := Inf {H | S ⊆ H}
+def closure (S : set G) : subgroup G := Inf {H | S ⊆ H}
 
 lemma mem_closure_iff {S : set G} {x : G} : 
-  x ∈ closure S ↔ ∀ H : subgroup2 G, S ⊆ H → x ∈ H := mem_bInter_iff
+  x ∈ closure S ↔ ∀ H : subgroup G, S ⊆ H → x ∈ H := mem_bInter_iff
 
 /- We will now prove some lemmas that are helpful in proving subgroups 
 form a galois_insertion with the coercion to set
@@ -211,7 +208,7 @@ form a galois_insertion with the coercion to set
 lemma le_closure (S : set G) : S ≤ closure S :=
 λ s hs H ⟨y, hy⟩, by rw ←hy; simp; exact λ hS, hS hs
 
-lemma closure_le (S : set G) (H : subgroup2 G) : closure S ≤ H ↔ S ⊆ H :=
+lemma closure_le (S : set G) (H : subgroup G) : closure S ≤ H ↔ S ⊆ H :=
 begin
   split,
     { intro h, refine subset.trans (le_closure _) h },
@@ -221,15 +218,15 @@ begin
       exact hy H h }
 end
 
-lemma closure_le' (S : set G) (H : subgroup2 G) : 
+lemma closure_le' (S : set G) (H : subgroup G) : 
   (closure S : set G) ⊆ H ↔ S ⊆ H := closure_le S H
 
-lemma closure_le'' (S : set G) (H : subgroup2 G) : 
+lemma closure_le'' (S : set G) (H : subgroup G) : 
   (∀ x, x ∈ closure S → x ∈ H) ↔ (∀ x, x ∈ S → x ∈ H) := closure_le S H
 
-lemma closure_self {H : subgroup2 G} : closure (H : set G) = H :=
+lemma closure_self {H : subgroup G} : closure (H : set G) = H :=
 begin
-  rw ←subgroup2.ext'_iff, ext,
+  rw ←subgroup.ext'_iff, ext,
   split; intro hx,
     { apply subset.trans _ ((closure_le (H : set G) H).2 (subset.refl H)), 
       exact hx, exact subset.refl _ },
@@ -250,14 +247,14 @@ by transfering the partial order on set to the partial order on subgroups.
 We do this because galois_insertion requires preorders and partial orders
 extends preoders.
 -/
-instance : partial_order (subgroup2 G) := 
-{.. partial_order.lift (coe : subgroup2 G → set G) (λ x y, subgroup2.ext')}
+instance : partial_order (subgroup G) := 
+{.. partial_order.lift (coe : subgroup G → set G) (λ x y, subgroup.ext')}
 
 /-
 Finially we prove that subgroups form a galois_insertion with the coercion 
 to set.
 -/
-def gi : galois_insertion (closure : set G → subgroup2 G) (coe : subgroup2 G → set G) :=
+def gi : galois_insertion (closure : set G → subgroup G) (coe : subgroup G → set G) :=
 { choice := λ S _, closure S,
   gc := λ H K,
     begin
@@ -271,10 +268,13 @@ def gi : galois_insertion (closure : set G → subgroup2 G) (coe : subgroup2 G �
 /-
 With that it follows that subgroup2s form a complete lattice!
 -/
-instance : complete_lattice (subgroup2 G) :=
+instance : complete_lattice (subgroup G) :=
 {.. galois_insertion.lift_complete_lattice gi}
 
-end subgroup2
+end subgroup
+
+end xena
+
 
 /-
 
